rocq/theories/TypeSystem/EnvRuntimeShadowEvalFacts.v
@@ -427,206 +427,6 @@ Proof.
     end.
 Qed.
 
-Lemma eval_expr_root_shadow_captured_call_provenance_summary_exact_preserves_typing :
-  forall env Ω n R Σ e T Σ' R' roots ret_roots,
-    expr_root_shadow_captured_call_provenance_summary_exact
-      env Ω n R Σ e T Σ' R' roots ret_roots ->
-    forall s s' ret,
-      store_typed env s Σ ->
-      store_roots_within R s ->
-      store_no_shadow s ->
-      root_env_no_shadow R ->
-      root_env_store_roots_named R s ->
-      root_env_store_keys_named R s ->
-      eval env s e s' ret ->
-      fn_env_unique_by_name env ->
-      store_typed env s' Σ' /\ value_has_type env s' ret T.
-Proof.
-  intros env Ω n R Σ e T Σ' R' roots ret_roots Hsummary.
-  induction Hsummary; intros s s' ret Hstore Hroots Hshadow Hrn Hnamed
-    Hkeys Heval Hunique.
-  - destruct (proj1 eval_preserves_typing_roots_ready_mutual
-        env s e s' ret Heval Ω n R Σ T Σ' R' roots
-        H Hstore Hroots Hshadow Hrn
-        (typed_env_roots_shadow_safe_roots
-          env Ω n R Σ e T Σ' R' roots H0))
-      as [Hstore' [Hv _]].
-    split; assumption.
-  - subst synthetic_body.
-    assert (Heval_call : eval env s (ECall fname args) s' ret).
-    { unfold direct_call_target_expr in H.
-      destruct e; try discriminate.
-      - inversion H; subst. exact Heval.
-      - destruct e; try discriminate.
-        inversion H; subst.
-        apply eval_call_expr_fn_as_call. exact Heval. }
-    destruct (eval_preserves_typing_direct_call_roots_provenance_ready_with_callee_summary
-        env s s' ret fname args Heval_call Ω n R Σ T Σ' R' roots
-        fcallee H1 Hstore Hroots Hshadow Hrn Hnamed Hkeys
-        (typed_env_roots_shadow_safe_roots
-          env Ω n R Σ (ECall fname args) T Σ' R' roots H6)
-        Hunique H2 H3 H4)
-      as [Hstore' [Hv _]].
-    split; assumption.
-  - assert (Hnodup_caps :
-        NoDup (ctx_names (params_ctx (fn_captures fcallee)))).
-    { match goal with
-      | Hnodup : NoDup (ctx_names
-          (params_ctx (fn_params fcallee ++ fn_captures fcallee))) |- _ =>
-          rewrite params_ctx_app, ctx_names_app in Hnodup;
-          eapply NoDup_app_right_ts; exact Hnodup
-      end. }
-    eapply eval_make_closure_captured_call_expr_shadow_preserves_typing_with_callee_components;
-      eauto.
-  - assert (Hnodup_caps :
-        NoDup (ctx_names (params_ctx (fn_captures fcallee)))).
-    { match goal with
-      | Hnodup : NoDup (ctx_names
-          (params_ctx (fn_params fcallee ++ fn_captures fcallee))) |- _ =>
-          rewrite params_ctx_app, ctx_names_app in Hnodup;
-          eapply NoDup_app_right_ts; exact Hnodup
-      end. }
-    rename x into x_hidden.
-    assert (Hfresh_s : ~ In x_hidden (store_names s)).
-    { apply store_lookup_none_not_in_store_names.
-      eapply store_roots_within_lookup_none; eassumption. }
-    dependent destruction H17.
-    { pose proof (lookup_fn_in_unique_by_name env (fn_name fdef) fdef
-                    H17 eq_refl Hunique) as Hlookup_direct.
-      pose proof (lookup_fn_in_unique_by_name env (fn_name fdef) fcallee
-                    H5 H6 Hunique) as Hlookup_callee.
-      rewrite Hlookup_direct in Hlookup_callee.
-      inversion Hlookup_callee; subst fdef.
-  		pose proof (typed_args_roots_shadow_safe_roots env Ω n R Σ args
-  		                  (apply_lt_params σ (fn_params fcallee))
-  		                  Σ' R' arg_roots H20)
-  		    as Htyped_args_roots.
-      destruct
-        (eval_let_make_closure_captured_call_expr_preserves_typing_with_callee_components_with_preservation_core
-          eval_preserves_typing_ready_mutual
-          eval_preserves_roots_ready_mutual
-          eval_preserves_root_names_ready_mutual
-          eval_preserves_root_keys_named_ready_mutual
-          eval_preserves_frame_scope_roots_ready_mutual
-          (eval_preserves_typing_roots_ready_prefix_mutual_statement_to_package
-            eval_preserves_typing_roots_ready_prefix_mutual)
-          eval_preserves_param_scope_roots_ready_mutual
-  	        env Ω n R Σ m x_hidden T_hidden args (fn_name fcallee) captures fcallee σ s s' ret
-  	        R' Σ' arg_roots env_lt captured_tys T_body Γ_out R_body
-          roots_body Hstore Hroots Hshadow Hrn Hnamed Hkeys H Heval H8
-          Hnodup_caps H4 Htyped_args_roots H9 H10 H11 H12 H13 H14
-          Hlookup_direct Hfresh_s H1 H2 H3)
-        as [Hstore' [Hv _]].
-      split.
-      + exact Hstore'.
-  	    + eapply VHT_Compatible.
-        * exact Hv.
-        * apply ty_compatible_b_sound. exact H22. }
-    (* TERS_CallExpr_Fn with EMakeClosure: impossible, guard violated *)
-    exfalso.
-    match goal with
-    | Hn : forall fn cs, EMakeClosure ?fname ?caps <> EMakeClosure fn cs |- _ =>
-        exact (Hn fname caps eq_refl)
-    end.
-    (* TERS_CallExpr_Closure with EMakeClosure: impossible, guard violated *)
-    exfalso.
-    match goal with
-    | Hn : forall fn cs, EMakeClosure ?fname ?caps <> EMakeClosure fn cs |- _ =>
-        exact (Hn fname caps eq_refl)
-    end.
-    (* TERS_CallExpr_TypeForall with EMakeClosure: impossible, guard violated *)
-    exfalso.
-    match goal with
-    | Hn : forall fn cs, EMakeClosure ?fname ?caps <> EMakeClosure fn cs |- _ =>
-        exact (Hn fname caps eq_refl)
-    end.
-    (* TERS_CallExpr_MixedForall with EMakeClosure: impossible, guard violated *)
-    exfalso.
-    match goal with
-    | Hn : forall fn cs, EMakeClosure ?fname ?caps <> EMakeClosure fn cs |- _ =>
-        exact (Hn fname caps eq_refl)
-    end.
-    (* TERS_CallExpr_Forall_Fn with EMakeClosure: impossible, guard violated *)
-    exfalso.
-    match goal with
-    | Hn : forall fn cs, EMakeClosure ?fname ?caps <> EMakeClosure fn cs |- _ =>
-        exact (Hn fname caps eq_refl)
-    end.
-  - dependent destruction Heval.
-    + destruct (proj1 eval_preserves_typing_roots_ready_mutual
-          env s e1 s1 (VBool true) Heval1 Ω n R Σ T_cond Σ1 R1
-          roots_cond H Hstore Hroots Hshadow Hrn
-          (typed_env_roots_shadow_safe_roots
-            env Ω n R Σ e1 T_cond Σ1 R1 roots_cond H0))
-        as [Hstore1 [_ _]].
-      destruct (proj1 eval_preserves_roots_ready_mutual
-          env s e1 s1 (VBool true) Heval1 Ω n R Σ T_cond Σ1 R1
-          roots_cond H Hroots Hshadow Hrn
-          (typed_env_roots_shadow_safe_roots
-            env Ω n R Σ e1 T_cond Σ1 R1 roots_cond H0))
-        as [Hroots1 [_ [Hshadow1 Hrn1]]].
-      destruct (proj1 eval_preserves_root_names_ready_mutual
-          env s e1 s1 (VBool true) Heval1 Ω n R Σ T_cond Σ1 R1
-          roots_cond H Hstore Hroots Hshadow Hrn Hnamed
-          (typed_env_roots_shadow_safe_roots
-            env Ω n R Σ e1 T_cond Σ1 R1 roots_cond H0))
-        as [Hnamed1 _].
-      pose proof (proj1 eval_preserves_root_keys_named_ready_mutual
-          env s e1 s1 (VBool true) Heval1 Ω n R Σ T_cond Σ1 R1
-          roots_cond H Hstore Hroots Hshadow Hrn Hkeys
-          (typed_env_roots_shadow_safe_roots
-            env Ω n R Σ e1 T_cond Σ1 R1 roots_cond H0))
-        as Hkeys1.
-      destruct (IHHsummary1 s1 s2 v Hstore1 Hroots1 Hshadow1 Hrn1
-          Hnamed1 Hkeys1 Heval2 Hunique) as [Hstore2 Hv].
-      split.
-      * eapply store_typed_ctx_merge_left; eassumption.
-      * eapply value_has_type_if_left_result. exact Hv.
-    + destruct (proj1 eval_preserves_typing_roots_ready_mutual
-          env s e1 s1 (VBool false) Heval1 Ω n R Σ T_cond Σ1 R1
-          roots_cond H Hstore Hroots Hshadow Hrn
-          (typed_env_roots_shadow_safe_roots
-            env Ω n R Σ e1 T_cond Σ1 R1 roots_cond H0))
-        as [Hstore1 [_ _]].
-      destruct (proj1 eval_preserves_roots_ready_mutual
-          env s e1 s1 (VBool false) Heval1 Ω n R Σ T_cond Σ1 R1
-          roots_cond H Hroots Hshadow Hrn
-          (typed_env_roots_shadow_safe_roots
-            env Ω n R Σ e1 T_cond Σ1 R1 roots_cond H0))
-        as [Hroots1 [_ [Hshadow1 Hrn1]]].
-      destruct (proj1 eval_preserves_root_names_ready_mutual
-          env s e1 s1 (VBool false) Heval1 Ω n R Σ T_cond Σ1 R1
-          roots_cond H Hstore Hroots Hshadow Hrn Hnamed
-          (typed_env_roots_shadow_safe_roots
-            env Ω n R Σ e1 T_cond Σ1 R1 roots_cond H0))
-        as [Hnamed1 _].
-      pose proof (proj1 eval_preserves_root_keys_named_ready_mutual
-          env s e1 s1 (VBool false) Heval1 Ω n R Σ T_cond Σ1 R1
-          roots_cond H Hstore Hroots Hshadow Hrn Hkeys
-          (typed_env_roots_shadow_safe_roots
-            env Ω n R Σ e1 T_cond Σ1 R1 roots_cond H0))
-        as Hkeys1.
-      destruct (IHHsummary2 s1 s2 v Hstore1 Hroots1 Hshadow1 Hrn1
-          Hnamed1 Hkeys1 Heval2 Hunique) as [Hstore3 Hv].
-      assert (Htypes : Forall2 sctx_entry_type_eq Σ2 Σ3).
-      { eapply typed_env_structural_branch_type_eq.
-        - eapply typed_env_roots_structural.
-          eapply typed_env_roots_shadow_safe_roots.
-          eapply expr_root_shadow_captured_call_provenance_summary_exact_typed.
-          exact Hsummary1.
-        - eapply typed_env_roots_structural.
-          eapply typed_env_roots_shadow_safe_roots.
-          eapply expr_root_shadow_captured_call_provenance_summary_exact_typed.
-          exact Hsummary2. }
-      split.
-      * eapply store_typed_ctx_merge_right; eassumption.
-      * eapply value_has_type_if_right_result.
-        -- exact Hv.
-        -- exact H2.
-Unshelve.
-  all: eauto.
-Qed.
-
 Lemma eval_expr_root_shadow_captured_call_provenance_summary_exact_package :
   forall env Ω n R Σ e T Σ' R' roots ret_roots,
     expr_root_shadow_captured_call_provenance_summary_exact
@@ -778,6 +578,84 @@ Proof.
         exact (Hn fname caps eq_refl)
     end.
   - dependent destruction Heval.
+    destruct (proj1 eval_preserves_typing_roots_ready_mutual
+        env s e1 s1 v1 Heval1 Ω n R Σ T1 Σ1 R1 roots1 H Hstore
+        Hroots Hshadow Hrn
+        (typed_env_roots_shadow_safe_roots
+          env Ω n R Σ e1 T1 Σ1 R1 roots1 H0))
+      as [Hstore1 [Hv1 _]].
+    destruct (proj1 eval_preserves_roots_ready_mutual
+        env s e1 s1 v1 Heval1 Ω n R Σ T1 Σ1 R1 roots1 H
+        Hroots Hshadow Hrn
+        (typed_env_roots_shadow_safe_roots
+          env Ω n R Σ e1 T1 Σ1 R1 roots1 H0))
+      as [Hroots1_runtime [Hv1_roots [Hshadow1 Hrn1]]].
+    destruct (proj1 eval_preserves_root_names_ready_mutual
+        env s e1 s1 v1 Heval1 Ω n R Σ T1 Σ1 R1 roots1 H
+        Hstore Hroots Hshadow Hrn Hnamed
+        (typed_env_roots_shadow_safe_roots
+          env Ω n R Σ e1 T1 Σ1 R1 roots1 H0))
+      as [Hnamed1 Hroots1_named].
+    pose proof (proj1 eval_preserves_root_keys_named_ready_mutual
+        env s e1 s1 v1 Heval1 Ω n R Σ T1 Σ1 R1 roots1 H
+        Hstore Hroots Hshadow Hrn Hkeys
+        (typed_env_roots_shadow_safe_roots
+          env Ω n R Σ e1 T1 Σ1 R1 roots1 H0))
+      as Hkeys1.
+    assert (Hfresh_store : store_lookup x s1 = None)
+      by (eapply store_roots_within_lookup_none; eassumption).
+    assert (Hadd_pres :
+      store_ref_targets_preserved env s1 (store_add x T_hidden v1 s1))
+      by (apply store_add_fresh_ref_targets_preserved; exact Hfresh_store).
+    assert (Hstore_add :
+      store_typed env (store_add x T_hidden v1 s1)
+        (sctx_add x T_hidden m Σ1)).
+    { eapply store_typed_add_compatible.
+      - exact Hstore1.
+      - exact Hv1.
+      - apply ty_compatible_b_sound. exact H1.
+      - exact Hadd_pres. }
+    assert (Hadd_roots :
+      store_roots_within (root_env_add x roots1 R1)
+        (store_add x T_hidden v1 s1))
+      by (eapply store_add_roots_within; eassumption).
+    assert (Hadd_shadow : store_no_shadow (store_add x T_hidden v1 s1))
+      by (apply store_no_shadow_add; assumption).
+    assert (Hadd_rn : root_env_no_shadow (root_env_add x roots1 R1))
+      by (apply root_env_no_shadow_add; assumption).
+    assert (Hadd_named :
+      root_env_store_roots_named (root_env_add x roots1 R1)
+        (store_add x T_hidden v1 s1))
+      by (eapply root_env_store_roots_named_add_env_store_add; eassumption).
+    assert (Hadd_keys :
+      root_env_store_keys_named (root_env_add x roots1 R1)
+        (store_add x T_hidden v1 s1))
+      by (eapply root_env_store_keys_named_add_env_store_add; eassumption).
+    destruct (IHHsummary (store_add x T_hidden v1 s1) s2 v2
+        Hstore_add Hadd_roots Hadd_shadow Hadd_rn Hadd_named Hadd_keys
+        Heval2 Hunique)
+      as [Hstore2 [Hv2 [Hroots2_runtime [Hvalue_roots [Hshadow2 Hrn2]]]]].
+    assert (Hremove_names :
+      forall se, In se (store_remove x s2) -> se_name se <> x)
+      by (apply store_no_shadow_remove_no_name; exact Hshadow2).
+    assert (Hroots_removed :
+      store_roots_within (root_env_remove x R2) (store_remove x s2))
+      by (eapply store_remove_roots_within; eassumption).
+    assert (Hexclude_store : store_refs_exclude_root x (store_remove x s2)).
+    { eapply store_roots_exclude_root.
+      - exact Hroots_removed.
+      - exact H8.
+      - exact Hremove_names. }
+    repeat split.
+    + eapply store_typed_remove_excluding_root; eassumption.
+    + eapply value_has_type_runtime_rootless_store_any.
+      * exact Hv2.
+      * apply capture_ref_free_ty_b_runtime_rootless. exact H5.
+    + exact Hroots_removed.
+    + exact Hvalue_roots.
+    + apply store_no_shadow_remove. exact Hshadow2.
+    + apply root_env_no_shadow_remove. exact Hrn2.
+  - dependent destruction Heval.
     + destruct (proj1 eval_preserves_typing_roots_ready_mutual
           env s e1 s1 (VBool true) Heval1 Ω n R Σ T_cond Σ1 R1
           roots_cond H Hstore Hroots Hshadow Hrn
@@ -865,3 +743,28 @@ Proof.
 Unshelve.
   all: eauto.
 Qed.
+
+Lemma eval_expr_root_shadow_captured_call_provenance_summary_exact_preserves_typing :
+  forall env Ω n R Σ e T Σ' R' roots ret_roots,
+    expr_root_shadow_captured_call_provenance_summary_exact
+      env Ω n R Σ e T Σ' R' roots ret_roots ->
+    forall s s' ret,
+      store_typed env s Σ ->
+      store_roots_within R s ->
+      store_no_shadow s ->
+      root_env_no_shadow R ->
+      root_env_store_roots_named R s ->
+      root_env_store_keys_named R s ->
+      eval env s e s' ret ->
+      fn_env_unique_by_name env ->
+      store_typed env s' Σ' /\ value_has_type env s' ret T.
+Proof.
+  intros env Ω n R Σ e T Σ' R' roots ret_roots Hsummary
+    s s' ret Hstore Hroots Hshadow Hrn Hnamed Hkeys Heval Hunique.
+  destruct (eval_expr_root_shadow_captured_call_provenance_summary_exact_package
+    env Ω n R Σ e T Σ' R' roots ret_roots Hsummary s s' ret
+    Hstore Hroots Hshadow Hrn Hnamed Hkeys Heval Hunique)
+    as [Hstore' [Hv _]].
+  split; assumption.
+Qed.
+
